令 $f(x)=x\ln x-x$

则 $b\ln a-a\ln b=a-b \Leftrightarrow f\left( \frac{1}{a} \right)=f\left( \frac{1}{b} \right)$

可知 $f'(x)=\ln x$

$f'(x)>0, \; \forall x \in(1, +\infty)$ 所以 $f(x)$ 在 $(1, +\infty)$ 上单调递增

$f'(x)<0, \; \forall x \in(0, 1)$ 所以 $f(x)$ 在 $(0, 1)$ 上单调递减

又 $a\neq b$ 故 $\frac{1}{a}$ 与 $\frac{1}{b}$ 一个小于 $1$ 一个大于 $1$

不妨设 $\frac{1}{a}<1$ 且 $\frac{1}{b}>1$

令 $g(x)=f(x)-f(2-x), \quad x \in (0,1]$

$g'(x)=f'(x)+f'(2-x)=\ln x + \ln (2-x)=\ln \left( -(x-1)^{2}+1\right) < \ln 1 =0, \quad \forall x \in (0, 1)$

又有 $g(1)=0$

所以 $g(x)>0, \quad \forall x \in (0, 1)$

故 $g\left( \frac{1}{a} \right) = f\left( \frac{1}{a} \right)-f\left( 2-\frac{1}{a} \right)>0 \Rightarrow f\left( \frac{1}{a} \right)=f\left( \frac{1}{b} \right)>f\left( 2-\frac{1}{a} \right)$

而 $\frac{1}{b}, 2-\frac{1}{a} \in (1, +\infty)$

所以 $\frac{1}{b}>2-\frac{1}{a}$ 即 $\frac{1}{a}+\frac{1}{b}>2$